Fixes to data page spec.

verified/smcapi.s.dfy
@@ -1,6 +1,7 @@
 include "kom_common.s.dfy"
 include "pagedb.s.dfy"
 include "entry.s.dfy"
+include "addrseq.dfy"
 
 predicate pageIsFree(d:PageDb, pg:PageNr)
 {
@@ -256,9 +257,10 @@ function smc_remove(pageDbIn: PageDb, page: word)
 }
 
 function smc_mapSecure(pageDbIn: PageDb, page: word, addrspacePage: word,
-    mapping: word, physPage: word, contents: seq<word>) : (PageDb, word) // PageDbOut, KOM_ERR
+    mapping: word, physPage: word, contents: Maybe<seq<word>>) : (PageDb, word) // PageDbOut, KOM_ERR
     requires validPageDb(pageDbIn)
-    requires |contents| == PAGESIZE / WORDSIZE
+    requires physPageIsInsecureRam(physPage) ==> contents.Just?
+    requires contents.Just? ==> |fromJust(contents)| == PAGESIZE / WORDSIZE
 {
     reveal_validPageDb();
     if(!isAddrspace(pageDbIn, addrspacePage)) then
@@ -274,7 +276,7 @@ function smc_mapSecure(pageDbIn: PageDb, page: word, addrspacePage: word,
                 (pageDbIn, KOM_ERR_INVALID_PAGENO)
             else
                 var ap_ret := allocatePage(pageDbIn, page,
-                    addrspacePage, DataPage(contents));
+                    addrspacePage, DataPage(fromJust(contents)));
                 var pageDbA := ap_ret.0;
                 var errA := ap_ret.1;
                 if(errA != KOM_ERR_SUCCESS) then (pageDbIn, errA)
@@ -331,40 +333,27 @@ function smc_stop(pageDbIn: PageDb, addrspacePage: word)
         (d', KOM_ERR_SUCCESS)
 }
 
-// Addr specialized version of range function in Seq.dfy that increments by 
-// WORDSIZE
-function addrSeq(l: addr, r: addr) : seq<addr>
-    requires isUInt32(l) && WordAligned(l) &&
-        isUInt32(r) && WordAligned(r)
-    requires l <= r
-    ensures |addrSeq(l, r)| == (r-l) / WORDSIZE
-    ensures forall i : addr | 0 <= i < r-l :: SeqOfNumbersInRightExclusiveRange(l, r)[i] == l + i
-    decreases r-l
-{
-    assert l+WORDSIZE > l;
-    assert r - (l+WORDSIZE) < r - l;
-    if l == r then [] else [l] + addrSeq(l+WORDSIZE,r)
-}
-
-function contentsOfPage(s: state, physPage: word) : seq<word>
+function contentsOfPage_(s: state, physPage: word) : seq<word>
     requires ValidState(s)
-    ensures |contentsOfPage(s, physPage)| == PAGESIZE / WORDSIZE
+    requires physPageIsInsecureRam(physPage)
+    ensures |contentsOfPage_(s, physPage)| == PAGESIZE / WORDSIZE
 {
     reveal_ValidMemState();
     var mem := s.m.addresses;
-    // TODO require this and make a monad-wrapped version
-    assume physPageIsInsecureRam(physPage);
     var base := physPage * PAGESIZE + KOM_DIRECTMAP_VBASE;
-    assert |addrSeq(base,base+PAGESIZE)| == PAGESIZE / WORDSIZE;
-    // Note: lambdas can't have refinement types so I can't write 
-    // a | a in mem => mem[a]. We have the same problem if we pass
-    // a => MemContents(s.m, a) as the lambda.
-    // Using a IMapSeqToSeq doesn't work since only the word-aligned
-    // part of the domain of addrSeq(...) is defined.
-    // I think this is okay, but I'm not sure how we 
-    // can make sure that it's okay.
-    MapSeqToSeq(addrSeq(base,base+PAGESIZE), 
-        a => if a in mem then mem[a] else 0)
+    assert |addrRangeSeq(base,base+PAGESIZE)| == PAGESIZE / WORDSIZE;
+    addrSeqToContents(addrsInPhysPage(physPage, base), mem)
+}
+
+function contentsOfPage(s: state, physPage: word) : Maybe<seq<word>>
+    requires ValidState(s)
+    ensures physPageIsInsecureRam(physPage) ==> contentsOfPage(s,physPage).Just?
+    ensures physPageIsInsecureRam(physPage) ==> 
+        |fromJust(contentsOfPage(s, physPage))| == PAGESIZE / WORDSIZE
+{
+    if(physPageIsInsecureRam(physPage)) then
+        Just(contentsOfPage_(s, physPage))
+    else Nothing
 }
 
 //=============================================================================
